src/program_proof/simplepb/pb_roapply_proof.v
@@ -6,10 +6,11 @@ From Perennial.goose_lang.lib Require Import waitgroup.
 From iris.base_logic Require Export lib.ghost_var mono_nat.
 From iris.algebra Require Import dfrac_agree mono_list.
 From Perennial.goose_lang Require Import crash_borrow.
-From Perennial.program_proof.simplepb Require Import pb_definitions pb_marshal_proof pb_applybackup_proof.
+From Perennial.program_proof.simplepb Require Import pb_definitions pb_marshal_proof pb_applybackup_proof pb_apply_proof.
+(* FIXME: importing apply_proof for some lemmas *)
 From Perennial.program_proof.reconnectclient Require Import proof.
 
-Section pb_apply_proof.
+Section pb_roapply_proof.
 
 Context `{!heapGS Σ}.
 Context {pb_record:PBRecord}.
@@ -135,7 +136,7 @@ Qed.
 
 Local Hint Rewrite get_rwops_single_nil.
 
-Lemma wp_Server__RoApply_internal (s:loc) γ γsrv op_sl op_bytes op Q :
+Lemma wp_Server__ApplyRo_internal (s:loc) γ γsrv op_sl op_bytes op Q :
   {{{
         is_Server s γ γsrv ∗
         readonly (is_slice_small op_sl byteT 1 op_bytes) ∗
@@ -548,60 +549,12 @@ Proof.
   { done. }
 Admitted.
 
-Lemma prefix_app_cases {A} (σ σ':list A) e:
-  σ' `prefix_of` σ ++ [e] →
-  σ' `prefix_of` σ ∨ σ' = (σ++[e]).
-Proof.
-  intros [σ0 Heq].
-  induction σ0 using rev_ind.
-  { rewrite app_nil_r in Heq. right; congruence. }
-  { rewrite app_assoc in Heq.
-    apply app_inj_2 in Heq as [-> ?]; last auto.
-    left. eexists; eauto.
-  }
-Qed.
-
-Lemma get_rwops_fst {A B} ops1 ops2 :
-  ops1.*1 = ops2.*1 →
-  get_rwops (A:=A) (pb_record:=pb_record) ops1 = get_rwops (A:=B) (pb_record:=pb_record) ops2.
-Proof.
-  intros.
-  revert dependent ops2.
-  induction ops1.
-  {
-    intros.
-    simpl.
-    destruct ops2.
-    { done. }
-    by exfalso.
-  }
-  intros.
-  revert dependent IHops1.
-  induction ops2; intros.
-  { by exfalso. }
-  replace (a :: ops1) with ([a] ++ ops1) in * by done.
-  replace (a0 :: ops2) with ([a0] ++ ops2) in * by done.
-  repeat rewrite get_rwops_app.
-  repeat rewrite fmap_app in H.
-  apply app_inj_1 in H; last done.
-  destruct H as [Hfirst Hrest].
-  injection Hfirst as Hfirst.
-  erewrite IHops1; last done.
-  f_equal.
-  destruct a, a0.
-  simpl in *.
-  unfold get_rwops.
-  simpl.
-  subst.
-  done.
-Qed.
-
-Lemma wp_Server__Apply (s:loc) γlog γ γsrv op_sl op (enc_op:list u8) Ψ (Φ: val → iProp Σ) :
+Lemma wp_Server__ApplyRo (s:loc) γlog γ γsrv op_sl op (enc_op:list u8) Ψ (Φ: val → iProp Σ) :
   is_Server s γ γsrv -∗
   readonly (is_slice_small op_sl byteT 1 enc_op) -∗
   (∀ reply, Ψ reply -∗ ∀ reply_ptr, ApplyReply.own_q reply_ptr reply -∗ Φ #reply_ptr) -∗
-  Apply_core_spec γ γlog op enc_op Ψ -∗
-  WP (pb.Server__Apply #s (slice_val op_sl)) {{ Φ }}
+  ApplyRo_core_spec γ γlog op enc_op Ψ -∗
+  WP (pb.Server__ApplyRo #s (slice_val op_sl)) {{ Φ }}
 .
 Proof using Type*.
   iIntros "#Hsrv #Hop_sl".
@@ -610,14 +563,14 @@ Proof using Type*.
   iDestruct "HΦ" as "(%Hop_enc & #Hinv & #Hupd & Hfail_Φ)".
   iMod (ghost_var_alloc (())) as (γtok) "Htok".
   set (OpPred :=
-(λ ops, inv escrowN (
+       (λ ops, inv escrowN (
         Ψ (ApplyReply.mkC 0 (compute_reply ops op)) ∨
           ghost_var γtok 1 ()
         ))).
 
   iMod (saved_pred_alloc OpPred DfracDiscarded) as (γghost_op) "#Hsaved"; first done.
   iApply wp_fupd.
-  wp_apply (wp_Server__Apply_internal _ _ _ _ _
+  wp_apply (wp_Server__ApplyRo_internal _ _ _ _ _
       op γghost_op
              with "[$Hsrv $Hop_sl Hupd]").
   {
@@ -641,17 +594,6 @@ Proof using Type*.
     destruct Hvalid as [_ <-].
     iExists _; iFrame.
     iIntros "Hghost".
-    iMod (own_update_2 with "Hlog Hlog2") as "Hlog".
-    {
-      rewrite -mono_list_auth_dfrac_op.
-      rewrite dfrac_op_own.
-      rewrite Qp.half_half.
-      apply mono_list_update.
-      instantiate (1:=_ ++ [op]).
-      by apply prefix_app_r.
-    }
-    iEval (rewrite -Qp.half_half -dfrac_op_own mono_list_auth_dfrac_op) in "Hlog".
-    iDestruct "Hlog" as "[Hlog Hlog2]".
     iMod ("Hupd" with "Hlog2") as "Hupd".
 
     iAssert (|={↑escrowN}=> inv escrowN ((Ψ (ApplyReply.mkC 0 (compute_reply (get_rwops opsfullQ) op)))
@@ -680,7 +622,7 @@ Proof using Type*.
     iMod ("Hclose" with "[HQs Hghost Hlog]").
     {
       iNext.
-      iExists (opsfullQ ++ [(rw_op op, OpPred)]); iFrame.
+      iExists (opsfullQ ++ [(ro_op op, OpPred)]); iFrame.
       iSplitL "Hghost".
       { iExists _. iFrame.
         iSplitL.
@@ -690,6 +632,8 @@ Proof using Type*.
         iApply big_sepL2_singleton. iFrame "Hsaved".
       }
       rewrite get_rwops_app.
+      rewrite get_rwops_single_nil.
+      rewrite app_nil_r.
       iFrame.
 
       iModIntro.
@@ -823,4 +767,4 @@ Proof using Type*.
   }
 Qed.
 
-End pb_apply_proof.
+End pb_roapply_proof.
